lean/Runtime/VM/Model.lean
@@ -9,6 +9,7 @@ import Runtime.VM.Model.Config
 import Runtime.VM.Model.CompileLocalTypeR
 import Runtime.VM.Model.Program
 import Runtime.VM.Model.Effects
+import Runtime.VM.Model.EffectsLemmas
 import Runtime.VM.Model.SemanticObjects
 import Runtime.VM.Model.State
 import Runtime.VM.Model.UnitModel
